src/lang/Thread.v
@@ -1,42 +1,206 @@
-Require Import sflib.
+Require Import Omega.
+Require Import RelationClasses.
 
+Require Import sflib.
+Require Import paco.
+
+Require Import Axioms.
 Require Import Basic.
+Require Import DataStructure.
 Require Import Event.
 Require Import Time.
+Require Import Language.
+Require Import Memory.
 
 Set Implicit Arguments.
 
-Module Language.
+
+Module Commit.
   Structure t := mk {
-    syntax: Type;
-    state: Type;
-
-    init: syntax -> state;
-    is_terminal: state -> Prop;
-    step: forall (s1:state) (e:option ThreadEvent.t) (s2:state), Prop;
-  }.
-End Language.
-
-Module ThreadState.
-  Structure syntax := mk_syntax {
-    syntax_lang: Language.t;
-    syntax_syntax: syntax_lang.(Language.syntax);
+    current: Snapshot.t;
+    released: LocFun.t Snapshot.t;
+    acquirable: Snapshot.t;
   }.
 
+  Definition init: t := mk Snapshot.init (LocFun.init Snapshot.init) Snapshot.init.
+
+  Inductive le (lhs rhs:t): Prop :=
+  | le_intro
+      (CURRENT: Snapshot.le lhs.(current) rhs.(current))
+      (RELEASED: forall (loc:Loc.t), Snapshot.le (LocFun.find loc lhs.(released)) (LocFun.find loc rhs.(released)))
+      (ACQUIRABLE: Snapshot.le lhs.(acquirable) rhs.(acquirable))
+  .
+
+  Global Program Instance le_PreOrder: PreOrder le.
+  Next Obligation.
+    ii. econs; reflexivity.
+  Qed.
+  Next Obligation.
+    ii. inv H. inv H0. econs; etransitivity; eauto.
+  Qed.
+
+  Inductive read
+            (tc1:t) (loc:Loc.t) (ts:Time.t) (released:Snapshot.t) (ord:Ordering.t)
+            (tc2:t): Prop :=
+  | read_intro
+      (MONOTONE: le tc1 tc2)
+      (READABLE: Snapshot.readable tc1.(current) loc ts)
+      (READ: Time.le ts (Times.get loc tc2.(current).(Snapshot.reads)))
+      (ACQUIRE: forall (ORDERING: Ordering.le Ordering.acquire ord),
+          Snapshot.le released tc2.(current))
+      (ACQUIRABLE: Snapshot.le released tc2.(acquirable))
+  .
+
+  Inductive write
+            (tc1:t) (loc:Loc.t) (ts:Time.t) (released:Snapshot.t) (ord:Ordering.t)
+            (tc2:t): Prop :=
+  | write_intro
+      (MONOTONE: le tc1 tc2)
+      (WRITABLE: Snapshot.writable tc1.(current) loc ts)
+      (WRITE: Time.le ts (Times.get loc tc2.(current).(Snapshot.writes)))
+      (RELEASE: forall (ORDERING: Ordering.le Ordering.release ord),
+          Snapshot.le tc2.(current) released)
+      (RELEASED: Snapshot.le (LocFun.find loc tc2.(Commit.released)) released)
+  .
+
+  Inductive fence
+            (tc1:t) (ord:Ordering.t)
+            (tc2:t): Prop :=
+  | fence_intro
+      (MONOTONE: le tc1 tc2)
+      (ACQUIRE: forall (ORDERING: Ordering.le Ordering.acquire ord),
+          Snapshot.le tc2.(acquirable) tc2.(current))
+      (RELEASE: forall (ORDERING: Ordering.le Ordering.release ord) loc,
+          Snapshot.le tc2.(current) (LocFun.find loc tc2.(released)))
+  .
+End Commit.
+
+Module Thread.
   Structure t := mk {
-    lang: Language.t;
-    state: lang.(Language.state)
+    state: State.t;
+    commit: Commit.t;
+    local: Memory.t;
   }.
 
-  Definition init (s:syntax): t :=
-    mk s.(syntax_lang) (s.(syntax_lang).(Language.init) s.(syntax_syntax)).
+  Definition init (s:State.syntax) := mk (State.init s) Commit.init Memory.init.
 
-  Definition is_terminal (th:t): Prop :=
-    th.(lang).(Language.is_terminal) th.(state).
+  Definition is_terminal (th:t): Prop := State.is_terminal th.(state).
 
-  Inductive step: forall (t1:t) (e:option ThreadEvent.t) (t2:t), Prop :=
-  | step_intro
-      lang s1 e s2
-      (STEP: lang.(Language.step) s1 e s2):
-      step (mk lang s1) e (mk lang s2).
-End ThreadState.
+  Inductive memory_step (th1:t) (mem1:Memory.t): forall (th2:t), Prop :=
+  | step_read
+      loc val ts released ord st2 commit2
+      (STATE: State.step th1.(state) (Some (ThreadEvent.mem (MemEvent.read loc val ord))) st2)
+      (READ: Commit.read th1.(commit) loc ts released ord commit2)
+      (MESSAGE: Memory.get loc ts mem1 = Some (Message.mk val released))
+      (LOCAL: Memory.get loc ts th1.(local) = None):
+      memory_step th1 mem1
+                  (mk st2 commit2 th1.(local))
+  | step_write
+      loc val ts released ord st2 commit2
+      (STATE: State.step th1.(state) (Some (ThreadEvent.mem (MemEvent.write loc val ord))) st2)
+      (WRITE: Commit.write th1.(commit) loc ts released ord commit2)
+      (MESSAGE: Memory.get loc ts th1.(local) = Some (Message.mk val released)):
+      memory_step th1 mem1
+                  (mk st2 commit2 (Memory.remove loc ts th1.(local)))
+  | step_update
+      loc valr tsr releasedr valw tsw releasedw ord st3 commit2 commit3
+      (STATE: State.step th1.(state) (Some (ThreadEvent.mem (MemEvent.update loc valr valw ord))) st3)
+      (READ: Commit.read th1.(commit) loc tsr releasedr ord commit2)
+      (WRITE: Commit.write commit2 loc tsw releasedw ord commit3)
+      (RELEASE: Snapshot.le releasedr releasedw)
+      (MESSAGE1: Memory.get loc tsr mem1 = Some (Message.mk valr releasedr))
+      (MESSAGE2: Memory.get loc tsw th1.(local) = Some (Message.mk valw releasedw)):
+      memory_step th1 mem1
+                  (mk st3 commit3 (Memory.remove loc tsw th1.(local)))
+  | step_fence
+      ord st2 commit2
+      (STATE: State.step th1.(state) (Some (ThreadEvent.mem (MemEvent.fence ord))) st2)
+      (FENCE: Commit.fence th1.(commit) ord commit2):
+      memory_step th1 mem1
+                  (mk st2 commit2 th1.(local))
+  | step_None
+      commit2
+      (COMMIT: Commit.le th1.(commit) commit2):
+      memory_step th1 mem1
+                  (mk th1.(state) commit2 th1.(local))
+  .
+
+  Inductive declare_step (th1:t) (mem1:Memory.t) (th2:t) (mem2:Memory.t): Prop :=
+  | declare_step_intro
+      loc from to msg
+      (STATE: th1.(state) = th2.(state))
+      (COMMIT: Commit.le th1.(commit) th2.(commit))
+      (LOCAL: Memory.declare loc from to msg th1.(local) th2.(local))
+      (MEMORY: Memory.declare loc from to msg mem1 mem2)
+  .
+
+  Inductive step: forall (e:option Event.t) (th1:t) (mem1:Memory.t) (th2:t) (mem2:Memory.t), Prop :=
+  | step_memory
+      th1 th2 mem
+      (STEP: memory_step th1 mem th2):
+      step None th1 mem th2 mem
+  | step_declare
+      th1 mem1 th2 mem2
+      (STEP: declare_step th1 mem1 th2 mem2):
+      step None th1 mem1 th2 mem2
+  | step_external
+      st1 st2 commit1 commit2 mem e
+      (STATE: State.step st1 (Some (ThreadEvent.syscall e)) st2)
+      (COMMIT: Commit.le commit1 commit2):
+      step (Some e)
+           (mk st1 commit1 Memory.init) mem
+           (mk st2 commit2 Memory.init) mem
+  .
+
+  Inductive internal_step (c1 c2:t * Memory.t): Prop :=
+  | internal_step_intro
+      (STEP: step None c1.(fst) c1.(snd) c2.(fst) c2.(snd))
+  .
+
+  Definition consistent (th1:t) (mem:Memory.t): Prop :=
+    forall mem1
+      (LOCAL: Memory.le th1.(Thread.local) mem1)
+      (FUTURE: Memory.future mem mem1),
+    exists th2 mem2,
+      <<STEPS: rtc internal_step (th1, mem1) (th2, mem2)>> /\
+      <<DECLARE: th2.(Thread.local) = Memory.init>>.
+
+  Lemma disjoint_memory_step
+        th1 mem1 th2 mem_o
+        (STEP: memory_step th1 mem1 th2)
+        (DISJOINT: Memory.disjoint mem_o th1.(local))
+        (LE: Memory.le mem_o mem1):
+    Memory.disjoint mem_o th2.(local).
+  Proof.
+    inv STEP; simpl in *; auto.
+    - admit.
+    - admit.
+  Admitted.
+
+  Lemma disjoint_declare_step
+        th1 mem1 th2 mem2 mem_o
+        (STEP: declare_step th1 mem1 th2 mem2)
+        (DISJOINT: Memory.disjoint mem_o th1.(local))
+        (LE: Memory.le mem_o mem1):
+    <<DISJOINT: Memory.disjoint mem_o th2.(local)>> /\
+    <<LE: Memory.le mem_o mem2>>.
+  Proof.
+    inv STEP.
+    admit.
+  Admitted.
+
+  Lemma disjoint_step
+        th1 mem1 th2 mem2 e mem_o
+        (STEP: step e th1 mem1 th2 mem2)
+        (DISJOINT: Memory.disjoint mem_o th1.(local))
+        (LE: Memory.le mem_o mem1):
+    <<DISJOINT: Memory.disjoint mem_o th2.(local)>> /\
+    <<LE: Memory.le mem_o mem2>>.
+  Proof.
+    inv STEP.
+    - splits; auto.
+      eapply disjoint_memory_step; eauto.
+    - eapply disjoint_declare_step; eauto.
+    - simpl in *. splits; auto.
+  Qed.
+End Thread.
