src/opt/Reorder.v
@@ -7,9 +7,12 @@ Require Import paco.
 
 Require Import Basic.
 Require Import Event.
+Require Import Language.
+Require Import Memory.
 Require Import Thread.
-Require Import ConfigurationRR.
+Require Import Configuration.
 Require Import Simulation.
+
 Require Import Syntax.
 Require Import Semantics.
 
@@ -18,277 +21,22 @@ Set Implicit Arguments.
 (* TODO: now supporting only the reordering of load and store *)
 (* TODO: now supporting only the reordering of single thread *)
 
-Inductive reordered_instr: forall (i1 i2:Instr.t), Prop :=
-| reordered_instr_load_store
+Inductive reorder: forall (i1 i2:Instr.t), Prop :=
+| reorder_load_store
     r1 l1 o1
     l2 v2 o2
     (LOC: l1 <> l2)
     (DISJOINT: RegSet.disjoint (Instr.regs_of (Instr.load r1 l1 o1)) (Instr.regs_of (Instr.store l2 v2 o2)))
     (ORDERING1: ~ Ordering.le Ordering.acquire o1)
     (ORDERING1: ~ Ordering.le Ordering.release o2):
-    reordered_instr (Instr.load r1 l1 o1) (Instr.store l2 v2 o2)
+    reorder (Instr.load r1 l1 o1) (Instr.store l2 v2 o2)
 .
 
-Inductive reordered_stmt: forall (s1 s2:Stmt.t), Prop :=
-| reordered_stmt_instr i:
-    reordered_stmt
-      (Stmt.instr i)
-      (Stmt.instr i)
-| reordered_stmt_ite
-    cond c11 c12 c21 c22
-    (REORDER1: reordered_stmts c11 c21)
-    (REORDER2: reordered_stmts c12 c22):
-    reordered_stmt
-      (Stmt.ite cond c11 c12)
-      (Stmt.ite cond c21 c22)
-| reordered_stmt_dowhile
-    cond c1 c2
-    (REORDER2: reordered_stmts c1 c2):
-    reordered_stmt
-      (Stmt.dowhile c1 cond)
-      (Stmt.dowhile c2 cond)
-
-with reordered_stmts: forall (s1 s2:list Stmt.t), Prop :=
-| reordered_stmts_nil:
-    reordered_stmts nil nil
-| reordered_stmts_cons
-    s11 s12 s21 s22
-    (REORDER1: reordered_stmt s11 s21)
-    (REORDER2: reordered_stmts s12 s22):
-    reordered_stmts (s11::s12) (s21::s22)
-| reordered_stmts_reorder
-    i1 i2 s1 s2
-    (REORDER: reordered_instr i1 i2)
-    (REORDER: reordered_stmts s1 s2):
-    reordered_stmts
-      ((Stmt.instr i1)::(Stmt.instr i2)::s1)
-      ((Stmt.instr i2)::(Stmt.instr i1)::s2)
-.
-
-Scheme reordered_stmt_ind_ := Induction for reordered_stmt Sort Prop
-with reordered_stmts_ind_ := Induction for reordered_stmts Sort Prop.
-Combined Scheme reordered_ind from reordered_stmt_ind_, reordered_stmts_ind_.
-
-Inductive reordered_thread: forall (text1 text2:Thread.syntax), Prop :=
-| reordered_thread_intro
-    s1 s2
-    (REORDER: reordered_stmts s1 s2):
-    reordered_thread
-      (Thread.mk_syntax lang s1)
-      (Thread.mk_syntax lang s2)
-.
-
-Inductive reordered_program tid: forall (prog1 prog2:Configuration.syntax), Prop :=
-| reordered_program_intro
-    prog1 th1 th2
-    (TH1: IdentMap.find tid prog1 = Some th1)
-    (REORDER: reordered_thread th1 th2):
-    reordered_program tid prog1 (IdentMap.add tid th2 prog1)
-.
-
-Inductive sim_reordered_thread: forall (th1 th2:Thread.t), Prop :=
-| sim_reordered_thread_intro
-    rs s1 s2
-    (REORDER: reordered_stmts s1 s2):
-    sim_reordered_thread
-      (Thread.mk lang (State.mk rs s1))
-      (Thread.mk lang (State.mk rs s2))
-.
-
-(* TODO: refactoring *)
-Lemma sim_reordered_thread_inv
-      th1 th2 (SIM: sim_reordered_thread th1 th2):
-  exists rs s1 s2,
-    th1 = Thread.mk lang (State.mk rs s1) /\
-    th2 = Thread.mk lang (State.mk rs s2) /\
-    reordered_stmts s1 s2.
-Proof.
-  inv SIM. eexists _, _, _. splits; eauto.
-Qed.
-
-Inductive sim_consumed_thread (e:option MemEvent.t): forall (th1 th2' th2:Thread.t), Prop :=
-| sim_consumed_thread_intro
-    i1 i2 rs1 rs2 s1 s2 tid
-    (REORDER: reordered_instr i1 i2)
-    (REORDER: reordered_stmts s1 s2)
-    (EVAL: RegFile.eval_instr rs1 tid (option_map ThreadEvent.mem e) rs2):
-    sim_consumed_thread
-      e
-      (Thread.mk lang (State.mk rs1 ((Stmt.instr i1)::(Stmt.instr i2)::s1)))
-      (Thread.mk lang (State.mk rs1 ((Stmt.instr i2)::(Stmt.instr i1)::s2)))
-      (Thread.mk lang (State.mk rs2 ((Stmt.instr i1)::s2)))
-.
-
-(* TODO: refactoring *)
-Lemma sim_consumed_thread_inv
-      e th1 th2' th2 (SIM: sim_consumed_thread e th1 th2' th2):
-  exists i1 i2 rs1 rs2 s1 s2 tid,
-    th1 = Thread.mk lang (State.mk rs1 ((Stmt.instr i1)::(Stmt.instr i2)::s1)) /\
-    th2' = Thread.mk lang (State.mk rs1 ((Stmt.instr i2)::(Stmt.instr i1)::s2)) /\
-    th2 = Thread.mk lang (State.mk rs2 ((Stmt.instr i1)::s2)) /\
-    reordered_instr i1 i2 /\
-    reordered_stmts s1 s2 /\
-    RegFile.eval_instr rs1 tid (option_map ThreadEvent.mem e) rs2.
-Proof.
-  inv SIM. eexists _, _, _, _, _, _, _. splits; eauto.
-Qed.
-
-Inductive sim_thread m1 m2 commit1 commit2 th1 th2: Prop :=
-| sim_thread_reordered
-    (TH: sim_reordered_thread th1 th2)
-    (MESSAGES: m1 = m2)
-    (COMMIT: commit1 = commit2)
-| sim_thread_consumed
-    th2' reading e
-    (TH: sim_consumed_thread e th1 th2' th2)
-    (MESSAGES: Commit.step commit1 m1 reading e commit2 m2)
-.
-
-Inductive sim_configuration (tid:Ident.t) (conf1 conf2:Configuration.t): Prop :=
-| sim_configuration_intro
-    commit1 commit2 th1 th2
-    (CONTEXT: forall i (TID: i <> tid),
-        IdentMap.find i conf1.(Configuration.threads) = IdentMap.find i conf2.(Configuration.threads))
-    (TH1: IdentMap.find tid conf1.(Configuration.threads) = Some (commit1, th1))
-    (TH2: IdentMap.find tid conf2.(Configuration.threads) = Some (commit2, th2))
-    (TH: sim_thread conf1.(Configuration.messages) conf2.(Configuration.messages) commit1 commit2 th1 th2)
-.
-
-Lemma sim_init
-      tid prog_src prog_tgt
-      (REORDER: reordered_program tid prog_src prog_tgt):
-  Simulation.INIT (sim_configuration tid) prog_src prog_tgt.
-Proof.
-  inv REORDER. unfold Simulation.INIT, Configuration.init.
-  econs; simpl; eauto.
-  - i. rewrite ? IdentMap.Facts.map_o.
-    rewrite IdentMap.Facts.add_neq_o; auto.
-  - rewrite IdentMap.Facts.map_o.
-    rewrite TH1. simpl. eauto.
-  - rewrite IdentMap.Facts.map_o.
-    rewrite IdentMap.Facts.add_eq_o; auto. simpl. eauto.
-  - inv REORDER0. econs; eauto. econs; eauto.
-Qed.
-
-Lemma sim_consistent tid: Simulation.CONSISTENT (sim_configuration tid).
-Proof.
-  ii. inv SIM. inv TH.
-  - econs.
-    + econs 1.
-    + rewrite MESSAGES. auto.
-  - admit. (* consumed *)
-Admitted.
-
-Lemma sim_base tid: Simulation.BASE_STEP (sim_configuration tid).
-Proof.
-  ii. inv SIM. inv TH.
-  - (* reordered *)
-    inv STEP.
-    + (* thread *)
-      admit.
-    + (* declare *)
-      eexists _, _. splits; eauto.
-      * apply Configuration.step_confirmed.
-        eapply Configuration.step_declare.
-        rewrite MESSAGES. eauto.
-      * econs; eauto. apply sim_thread_reordered; eauto.
-    + (* commit *)
-      destruct (Ident.eq_dec tid0 tid).
-      * subst. rewrite TH2 in TID. inv TID.
-        eexists _, _. splits; eauto.
-        { apply Configuration.step_confirmed.
-          eapply Configuration.step_commit; eauto.
-        }
-        { econs; simpl; eauto.
-          - i. rewrite ? IdentMap.Facts.add_neq_o; eauto.
-          - rewrite IdentMap.Facts.add_eq_o; eauto.
-          - rewrite IdentMap.Facts.add_eq_o; eauto.
-          - apply sim_thread_reordered; eauto.
-        }
-      * exploit CONTEXT; eauto. intro X.
-        eexists _, _. splits; eauto.
-        { apply Configuration.step_confirmed.
-          eapply Configuration.step_commit; [|eauto].
-          rewrite X. eauto.
-        }
-        { econs; simpl; eauto.
-          - i. rewrite ? IdentMap.Facts.add_o.
-            destruct (IdentMap.Facts.eq_dec tid0 i); eauto.
-          - rewrite IdentMap.Facts.add_neq_o; eauto.
-          - rewrite IdentMap.Facts.add_neq_o; eauto.
-          - apply sim_thread_reordered; eauto.
-        }
-  - (* consumed *)
-    inv STEP.
-    + (* thread *)
-      admit.
-    + (* declare *)
-      admit.
-    + (* commit *)
-      destruct (Ident.eq_dec tid0 tid).
-      * subst. rewrite TH2 in TID. inv TID.
-        eexists _, _. splits; eauto.
-        { apply Configuration.step_confirmed.
-          eapply Configuration.step_commit; eauto.
-          admit.
-        }
-        { econs; simpl; eauto.
-          - i. rewrite ? IdentMap.Facts.add_neq_o; eauto.
-          - rewrite IdentMap.Facts.add_eq_o; eauto.
-          - rewrite IdentMap.Facts.add_eq_o; eauto.
-          - apply sim_thread_reordered; eauto.
-            admit.
-            admit.
-        }
-      * exploit CONTEXT; eauto. intro X.
-        eexists _, _. splits; eauto.
-        { apply Configuration.step_confirmed.
-          eapply Configuration.step_commit; [|eauto].
-          rewrite X. eauto.
-        }
-        { econs; simpl; eauto.
-          - i. rewrite ? IdentMap.Facts.add_o.
-            destruct (IdentMap.Facts.eq_dec tid0 i); eauto.
-          - rewrite IdentMap.Facts.add_neq_o; eauto.
-          - rewrite IdentMap.Facts.add_neq_o; eauto.
-          - apply sim_thread_reordered; eauto.
-            admit.
-            admit.
-            admit.
-        }
-Admitted.
-
-Lemma sim_external tid: Simulation.EXTERNAL_STEP (sim_configuration tid).
+Lemma reorder_sim_thread
+      i1 i2
+      (REORDER: reorder i1 i2):
+  sim_thread_init
+    (State.mk_syntax lang [Stmt.instr i1; Stmt.instr i2])
+    (State.mk_syntax lang [Stmt.instr i2; Stmt.instr i1]).
 Proof.
 Admitted.
-
-Lemma sim_terminal tid: Simulation.TERMINAL (sim_configuration tid).
-Proof.
-  ii. eexists. split.
-  { econs 1. }
-  econs. i. inv TERM. specialize (TERMINAL tid0).
-  destruct (Ident.eq_dec tid0 tid); subst.
-  - inv SIM. rewrite FIND in TH1. inv TH1.
-    exploit TERMINAL; eauto. inv TH.
-    + inv TH0.
-      unfold Thread.is_terminal. simpl.
-      unfold State.is_terminal. simpl.
-      inv REORDER; congruence.
-    + inv TH0.
-      unfold Thread.is_terminal. simpl.
-      unfold State.is_terminal. simpl.
-      congruence.
-  - inv SIM. exploit CONTEXT; eauto. intro FIND0.
-    eapply TERMINAL. rewrite <- FIND0. eauto.
-Qed.
-
-Lemma sim tid:
-  reordered_program tid <2= Simulation.t.
-Proof.
-  i. eapply Simulation.sim_lemma.
-  - apply sim_init. eauto.
-  - apply sim_consistent.
-  - apply sim_base.
-  - apply sim_external.
-  - apply sim_terminal.
-Qed.
