src/opt/Simulation.v
@@ -3,136 +3,67 @@ Require Import paco.
 
 Require Import Basic.
 Require Import Event.
+Require Import Language.
+Require Import Memory.
 Require Import Thread.
 Require Import Configuration.
 
 Set Implicit Arguments.
 
-(* TODO: liveness *)
-Module Simulation.
-  Section Simulation.
-    Variable (sim: forall (src tgt:Configuration.t), Prop).
 
-    Definition INIT (prog_src prog_tgt:Configuration.syntax): Prop :=
-      sim (Configuration.init prog_src) (Configuration.init prog_tgt).
+Inductive sim_memory (mem_src mem_tgt:Memory.t): Prop :=
+| sim_memory_intro
+    (MESSAGES:
+       forall loc ts msg
+         (MSG: Memory.get loc ts mem_tgt = Some msg),
+         Memory.get loc ts mem_src = Some msg)
+    (OWNERSHIP: Memory.own mem_src = Memory.own mem_tgt)
+.
 
-    Definition STEP: Prop :=
-      forall src0 tgt0 e tgt2
-        (SIM: sim src0 tgt0)
-        (STEP: Configuration.step tgt0 e tgt2),
-      exists src1 src2,
-        <<INTERNAL: rtc Configuration.internal_step src0 src1>> /\
-        <<STEP: Configuration.step src1 e src2>> /\
-        <<SIM: sim src2 tgt2>>.
 
-    Definition TERMINAL: Prop :=
-      forall src0 tgt0
-        (SIM: sim src0 tgt0)
-        (TERM: Configuration.is_terminal tgt0),
-      exists src1,
-        <<INTERNAL: rtc Configuration.internal_step src0 src1>> /\
-        <<TERM: Configuration.is_terminal src1>>.
-  End Simulation.
+(* TODO: inftau & liveness *)
+Inductive _sim_thread
+          (sim_thread: forall (th1_src:Thread.t) (mem_k_src:Memory.t)
+                         (th1_tgt:Thread.t) (mem_k_tgt:Memory.t), Prop)
+          (th1_src:Thread.t) (mem_k_src:Memory.t)
+          (th1_tgt:Thread.t) (mem_k_tgt:Memory.t): Prop :=
+| sim_thread_terminal
+    (TGT: Thread.is_terminal th1_tgt)
+    (SRC: forall mem1_src
+            (LOCAL: Memory.le th1_src.(Thread.local) mem1_src)
+            (FUTURE: Memory.future mem_k_src mem1_src),
+        exists th2_src mem2_src,
+          <<STEPS: rtc Thread.internal_step (th1_src, mem1_src) (th2_src, mem2_src)>> /\
+          <<TERMINAL: Thread.is_terminal th2_src>>)
+| sim_thread_step
+    (STEP:
+       forall mem1_src mem1_tgt
+         (MEMORY1: sim_memory mem1_src mem1_tgt)
+         (LOCAL_SRC: Memory.le th1_src.(Thread.local) mem1_src)
+         (LOCAL_TGT: Memory.le th1_tgt.(Thread.local) mem1_tgt)
+         (FUTURE_SRC: Memory.future mem_k_src mem1_src)
+         (FUTURE_TGT: Memory.future mem_k_tgt mem1_tgt),
+       forall e th2_tgt mem2_tgt
+         (STEP_TGT: Thread.step e th1_tgt mem1_tgt th2_tgt mem2_tgt),
+       exists th2_src mem2_src,
+         <<STEP_SRC: Thread.step e th1_src mem1_src th2_src mem2_src>> /\
+         <<MEMORY2: sim_memory mem2_src mem2_tgt>> /\
+         <<SIM: sim_thread th2_src mem2_src th2_tgt mem2_tgt>>)
+.
+Hint Constructors _sim_thread.
 
-  Inductive t (prog_src prog_tgt:Configuration.syntax): Prop :=
-  | t_intro
-    sim
-    (I: INIT sim prog_src prog_tgt)
-    (S: STEP sim)
-    (T: TERMINAL sim)
-  .
+Lemma _sim_thread_mon: monotone4 _sim_thread.
+Proof.
+  repeat intro; inv IN.
+  - econs 1; eauto.
+  - econs 2. i.
+    exploit STEP; eauto. i. des.
+    eexists _, _. splits; eauto.
+Qed.
+Hint Resolve _sim_thread_mon: paco.
 
-  Section BaseSimulation.
-    Variable (sim: forall (src tgt:Configuration.t), Prop).
+Definition sim_thread: _ -> _ -> _ -> _ -> Prop := paco4 _sim_thread bot4.
 
-    Definition CONSISTENT: Prop :=
-      forall src tgt
-        (SIM: sim src tgt)
-        (CONFIRM: MessageSet.confirmed tgt.(Configuration.messages)),
-        Configuration.consistent src.
-
-    Definition BASE_STEP: Prop :=
-      forall src0 tgt0 reading tgt2
-        (SIM: sim src0 tgt0)
-        (STEP: Configuration.base_step tgt0 reading tgt2)
-        (READING:
-           forall loc ts (READING: reading = Some (loc, ts)),
-           exists (src0' tgt0':Configuration.t),
-             <<SIM: sim src0' tgt0'>> /\
-             <<SRC: rtc Configuration.internal_step src0 src0'>> /\
-             <<TGT: rtc Configuration.internal_step tgt0 tgt0'>> /\
-             <<DECLARE: MessageSet.declared tgt0'.(Configuration.messages) <2= MessageSet.declared tgt0.(Configuration.messages)>> /\
-             <<NODECLARE: ~ MessageSet.declared tgt0'.(Configuration.messages) loc ts>>),
-      exists src1 src2,
-        <<INTERNAL: rtc Configuration.internal_step src0 src1>> /\
-        <<STEP: Configuration.internal_step src1 src2>> /\
-        <<SIM: sim src2 tgt2>>.
-
-    Definition EXTERNAL_STEP: Prop :=
-      forall src0 tgt0 e tgt2
-        (SIM: sim src0 tgt0)
-        (STEP: Configuration.external_step tgt0 e tgt2),
-      exists src1 src2,
-        <<INTERNAL: rtc Configuration.internal_step src0 src1>> /\
-        <<STEP: Configuration.external_step src1 e src2>> /\
-        <<SIM: sim src2 tgt2>>.
-
-    Lemma internal_step (B:BASE_STEP):
-      forall src0 tgt0 tgt2
-        (SIM: sim src0 tgt0)
-        (STEP: Configuration.internal_step tgt0 tgt2),
-      exists src1 src2,
-        <<INTERNAL: rtc Configuration.internal_step src0 src1>> /\
-        <<STEP: Configuration.internal_step src1 src2>> /\
-        <<SIM: sim src2 tgt2>>.
-    Proof.
-      i. revert src0 SIM.
-      induction STEP0 using Configuration.internal_step_strong_ind; i.
-      - eapply B; eauto. congruence.
-      - eapply B; eauto. i. inv READING.
-        cut (exists src0', sim src0' c1' /\ rtc Configuration.internal_step src0 src0').
-        { i. des. eexists _, _. splits; eauto. }
-        revert src0 SIM. clear -PROP. induction PROP; i.
-        + eexists. splits; eauto.
-        + exploit H; eauto. i. des.
-          exploit IHPROP; eauto. i. des.
-          eexists. splits; eauto.
-          eapply rtc_trans; eauto.
-          econs 2; eauto.
-    Qed.
-
-    Lemma consistent (C:CONSISTENT) (B:BASE_STEP):
-      forall src0 tgt0
-        (SIM: sim src0 tgt0)
-        (TGT0: Configuration.consistent tgt0),
-        Configuration.consistent src0.
-    Proof.
-      i. inv TGT0. revert src0 SIM. induction STEPS; i.
-      - eapply C; eauto.
-      - exploit internal_step; eauto. i. des.
-        exploit IHSTEPS; eauto. intro X. inv X.
-        econs; [|eauto].
-        eapply rtc_trans; eauto.
-        econs 2; eauto.
-    Qed.
-
-    Lemma sim_lemma
-          (prog_src prog_tgt:Configuration.syntax)
-          (I:INIT sim prog_src prog_tgt)
-          (C:CONSISTENT) (B:BASE_STEP) (E:EXTERNAL_STEP)
-          (T:TERMINAL sim):
-      Simulation.t prog_src prog_tgt.
-    Proof.
-      econs; eauto.
-      ii. inv STEP0.
-      - exploit internal_step; eauto. i. des.
-        eexists _, _. splits; eauto.
-        econs; auto.
-        eapply consistent; eauto.
-      - exploit E; eauto. i. des.
-        eexists _, _. splits; eauto.
-        econs; auto.
-        eapply consistent; eauto.
-    Qed.
-  End BaseSimulation.
-End Simulation.
+Definition sim_thread_init s1 s2 :=
+  sim_thread (Thread.init s1) Memory.init
+             (Thread.init s2) Memory.init.
