src/lang/Language.v
@@ -1,0 +1,48 @@
+Require Import sflib.
+
+Require Import Basic.
+Require Import Event.
+Require Import Time.
+
+Set Implicit Arguments.
+
+Module Language.
+  Structure t := mk {
+    syntax: Type;
+    state: Type;
+
+    init: syntax -> state;
+    is_terminal: state -> Prop;
+    step: forall (s1:state) (e:option ThreadEvent.t) (s2:state), Prop;
+
+    IS_TERMINAL_STEP:
+      forall s1 e s2
+        (TERMINAL: is_terminal s1)
+        (STEP: step s1 e s2),
+        False;
+  }.
+End Language.
+
+Module State.
+  Structure syntax := mk_syntax {
+    syntax_lang: Language.t;
+    syntax_syntax: syntax_lang.(Language.syntax);
+  }.
+
+  Structure t := mk {
+    lang: Language.t;
+    state: lang.(Language.state)
+  }.
+
+  Definition init (s:syntax): t :=
+    mk s.(syntax_lang) (s.(syntax_lang).(Language.init) s.(syntax_syntax)).
+
+  Definition is_terminal (th:t): Prop :=
+    th.(lang).(Language.is_terminal) th.(state).
+
+  Inductive step: forall (t1:t) (e:option ThreadEvent.t) (t2:t), Prop :=
+  | step_intro
+      lang s1 e s2
+      (STEP: lang.(Language.step) s1 e s2):
+      step (mk lang s1) e (mk lang s2).
+End State.
